src/Narcissus/Examples/NetworkStack/ARPPacket.v
@@ -1,43 +1,49 @@
 Require Import
-        Coq.omega.Omega
         Coq.Strings.String
-        Coq.Vectors.Vector.
+        Coq.Vectors.Vector
+        Coq.omega.Omega.
 
 Require Import
+        Fiat.Common.SumType
+        Fiat.Common.EnumType
+        Fiat.Common.BoundedLookup
+        Fiat.Common.ilist
         Fiat.Computation
+        Fiat.QueryStructure.Specification.Representation.Notations
+        Fiat.QueryStructure.Specification.Representation.Heading
+        Fiat.QueryStructure.Specification.Representation.Tuple
+        Fiat.Narcissus.BinLib
         Fiat.Narcissus.Common.Specs
         Fiat.Narcissus.Common.WordFacts
+        Fiat.Narcissus.Common.ComposeCheckSum
         Fiat.Narcissus.Common.ComposeIf
         Fiat.Narcissus.Common.ComposeOpt
-        Fiat.Narcissus.Automation.Solver
-        Fiat.Narcissus.BinLib
         Fiat.Narcissus.Formats
-        Fiat.Narcissus.Stores.EmptyStore.
+        Fiat.Narcissus.BaseFormats
+        Fiat.Narcissus.Stores.EmptyStore
+        Fiat.Narcissus.Automation.Solver
+        Fiat.Narcissus.Automation.AlignedAutomation.
 
 Require Import Bedrock.Word.
 
 Import Vectors.VectorDef.VectorNotations.
-Open Scope string_scope.
-Open Scope Tuple_scope.
-
+Open Scope format_scope.
 Opaque pow2. (* Don't want to be evaluating this. *)
 Opaque natToWord. (* Or this. *)
 
-Definition monoid : Monoid ByteString := ByteStringQueueMonoid.
-
 (* Start Example Derivation. *)
 
-Definition ARPPacket :=
-  @Tuple <"HardType" :: EnumType ["Ethernet"; "802"; "Chaos"],
-          "ProtType" :: EnumType ["IPv4"; "IPv6"], (* Overlaps with etherType. *)
-          "Operation" :: EnumType ["Request";
-                                   "Reply";
-                                   "RARP Request";
-                                   "RARP Reply"],
-          "SenderHardAddress" :: list char,
-          "SenderProtAddress" :: list char,
-          "TargetHardAddress" :: list char,
-          "TargetProtAddress" :: list char >.
+Record ARPPacket :=
+  {HardType : EnumType ["Ethernet"; "802"; "Chaos"];
+   ProtType : EnumType ["IPv4"; "IPv6"]; (* Overlaps with etherType. *)
+   Operation : EnumType ["Request";
+                           "Reply";
+                           "RARP Request";
+                           "RARP Reply"];
+   SenderHardAddress : list (word 8);
+   SenderProtAddress : list (word 8);
+   TargetHardAddress : list (word 8);
+   TargetProtAddress : list (word 8)}.
 
 Definition HardTypeCodes : Vector.t (word 16) 3 :=
   [WO~0~0~0~0~0~0~0~0~0~0~0~0~0~0~0~1;
@@ -50,13 +56,13 @@ Definition EtherTypeCodes : Vector.t (word 16) 2 :=
    WO~1~0~0~0~0~1~1~0~1~1~0~1~1~1~0~1
   ].
 
-Definition HardSizeCodes : Vector.t char 3 :=
+Definition HardSizeCodes : Vector.t (word 8) 3 :=
   [WO~0~0~0~0~0~1~1~0;
    WO~0~0~0~0~0~1~1~0;
    WO~0~0~0~0~0~0~1~0
   ].
 
-Definition ProtSizeCodes : Vector.t char 2 :=
+Definition ProtSizeCodes : Vector.t (word 8) 2 :=
   [WO~0~0~0~0~0~1~0~0;
    WO~0~0~0~1~0~0~0~0 ].
 
@@ -67,32 +73,129 @@ Definition OperationCodes : Vector.t (word 16) 4 :=
    WO~0~0~0~0~0~0~0~0~0~0~0~0~0~1~0~0
   ].
 
-Definition format_ARPPacket_Spec (arp : ARPPacket) :=
-          format_enum HardTypeCodes arp!"HardType"
-    ThenC format_enum EtherTypeCodes arp!"ProtType"
-    ThenC format_word HardSizeCodes[@arp!"HardType"]
-    ThenC format_word ProtSizeCodes[@arp!"ProtType"]
-    ThenC format_enum OperationCodes arp!"Operation"
-    ThenC format_list format_word arp!"SenderHardAddress"
-    ThenC format_list format_word arp!"SenderProtAddress"
-    ThenC format_list format_word arp!"TargetHardAddress"
-    ThenC format_list format_word arp!"TargetProtAddress"
-    DoneC.
+Definition ARPPacket_Format
+  : FormatM ARPPacket ByteString :=
+  format_enum HardTypeCodes ◦ HardType
+    ++ format_enum EtherTypeCodes ◦ ProtType
+    ++ format_word ◦ (Basics.compose (Vector.nth HardSizeCodes) HardType)
+    ++ format_word ◦ (Basics.compose (Vector.nth ProtSizeCodes) ProtType)
+    ++ format_enum OperationCodes ◦ Operation
+    ++ format_list format_word ◦ SenderHardAddress
+    ++ format_list format_word ◦ SenderProtAddress
+    ++ format_list format_word ◦ TargetHardAddress
+    ++ format_list format_word ◦ TargetProtAddress.
 
 Definition ARP_Packet_OK (arp : ARPPacket) :=
-  (|arp!"SenderHardAddress"|) = wordToNat HardSizeCodes[@arp!"HardType"]
-  /\ (|arp!"SenderProtAddress"|) = wordToNat ProtSizeCodes[@arp!"ProtType"]
-  /\ (|arp!"TargetHardAddress"|) = wordToNat HardSizeCodes[@arp!"HardType"]
-  /\ (|arp!"TargetProtAddress"|) = wordToNat ProtSizeCodes[@arp!"ProtType"].
+  (|arp.(SenderHardAddress)|) = wordToNat HardSizeCodes[@arp.(HardType)]
+  /\ (|arp.(SenderProtAddress)|) = wordToNat ProtSizeCodes[@arp.(ProtType)]
+  /\ (|arp.(TargetHardAddress)|) = wordToNat HardSizeCodes[@arp.(HardType)]
+  /\ (|arp.(TargetProtAddress)|) = wordToNat ProtSizeCodes[@arp.(ProtType)].
 
 Arguments Vector.nth : simpl never.
 
-Definition ARPPacket_decoder
-  : CorrectDecoderFor ARP_Packet_OK format_ARPPacket_Spec.
+
+  (* Step One: Synthesize an encoder and a proof that it is correct. *)
+  Definition ARP_encoder :
+    CorrectAlignedEncoderFor ARPPacket_Format.
+  Proof.
+    start_synthesizing_encoder.
+    Ltac decompose_aligned_encoder :=
+      first [
+          eapply @CorrectAlignedEncoderForIPChecksumThenC
+        | associate_for_ByteAlignment
+        | apply @CorrectAlignedEncoderForThenC
+        | apply @CorrectAlignedEncoderForDoneC].
+    (decompose_aligned_encoder; eauto).
+    (decompose_aligned_encoder; eauto).
+    (decompose_aligned_encoder; eauto).
+    (decompose_aligned_encoder; eauto).
+    (decompose_aligned_encoder; eauto).
+    (decompose_aligned_encoder; eauto).
+    (decompose_aligned_encoder; eauto).
+    (decompose_aligned_encoder; eauto).
+    repeat align_encoder_step.
+    repeat align_encoder_step.
+    repeat align_encoder_step.
+    repeat align_encoder_step.
+    repeat align_encoder_step.
+    repeat align_encoder_step.
+    repeat align_encoder_step.
+    repeat align_encoder_step.
+    repeat align_encoder_step.
+    Grab Existential Variables.
+    eauto.
+    eauto.
+    eauto.
+    eauto.
+    eauto.
+    eauto.
+  Defined.
+
+  (* Step Two: Extract the encoder function, and have it start encoding
+   at the      start of the provided ByteString [v]. *)
+  Definition ARP_encoder_impl {sz} v r :=
+    Eval simpl in (projT1 ARP_encoder sz v 0 r tt).
+  Print ARP_encoder_impl.
+
+(* Step Three: Synthesize a decoder and a proof that /it/ is correct. *)
+Definition ARP_Packet_Header_decoder
+  : CorrectAlignedDecoderFor ARP_Packet_OK ARPPacket_Format.
 Proof.
-  synthesize_decoder.
+  (* We have to use an extra lemma at the start, because of the 'exotic'
+     IP Checksum. *)
+  start_synthesizing_decoder.
+  normalize_compose ByteStringQueueMonoid.
+  decode_step ltac:(idtac).
+  decode_step ltac:(idtac).
+  decode_step ltac:(idtac).
+  decode_step ltac:(idtac).
+  decode_step ltac:(idtac).
+  decode_step ltac:(idtac).
+  decode_step ltac:(idtac).
+  decode_step ltac:(idtac).
+  decode_step ltac:(idtac).
+  decode_step ltac:(idtac).
+  decode_step ltac:(idtac).
+  decode_step ltac:(idtac).
+  decode_step ltac:(idtac).
+  decode_step ltac:(idtac).
+  decode_step ltac:(idtac).
+  decode_step ltac:(idtac).
+  decode_step ltac:(idtac).
+  decode_step ltac:(idtac).
+  decode_step ltac:(idtac).
+  decode_step ltac:(idtac).
+  decode_step ltac:(idtac).
+  decode_step ltac:(idtac).
+  decode_step ltac:(idtac).
+  decode_step ltac:(idtac).
+  decode_step ltac:(idtac).
+  decode_step ltac:(idtac).
+  unfold ARP_Packet_OK; intros; intuition; rewrite H8 in H4; eassumption.
+  decode_step ltac:(idtac).
+  decode_step ltac:(idtac).
+  decode_step ltac:(idtac).
+  decode_step ltac:(idtac).
+  unfold ARP_Packet_OK; intros; intuition; rewrite H9 in H5; eassumption.
+  decode_step ltac:(idtac).
+  decode_step ltac:(idtac).
+  decode_step ltac:(idtac).
+  decode_step ltac:(idtac).
+  unfold ARP_Packet_OK; intros; intuition; rewrite H15, H12; reflexivity.
+  decode_step ltac:(idtac).
+  decode_step ltac:(idtac).
+  decode_step ltac:(idtac).
+  decode_step ltac:(idtac).
+  unfold ARP_Packet_OK; intros; intuition; rewrite H19, H13; reflexivity.
+  decode_step ltac:(idtac).
+  decode_step ltac:(idtac).
+  cbv beta; synthesize_cache_invariant.
+  cbv beta; unfold decode_nat; optimize_decoder_impl.
+  cbv beta; align_decoders.
 Defined.
 
-Definition ARP_Packet_decoder :=
-  Eval simpl in proj1_sig ARPPacket_decoder.
-Print ARP_Packet_decoder.
+(* Step Four: Extract the decoder function, and have /it/ start decoding
+   at the start of the provided ByteString [v]. *)
+Arguments GetCurrentBytes : simpl never.
+Definition ARP_decoder_impl {sz} v :=
+  Eval simpl in (projT1 ARP_Packet_Header_decoder sz v 0 ()).
